Use Hprop and Hpost

Semantic/FsubNext/Eval/BigStep.lean
@@ -4,19 +4,13 @@ import Semantic.FsubNext.Heap
 
 namespace FsubNext
 
-def pred_is_monotonic (pred : Heap -> Exp {} -> Prop) : Prop :=
-  ∀ {h1 h2 : Heap} {e},
-    h2.subsumes h1 ->
-    pred h1 e ->
-    pred h2 e
-
-inductive Eval : Heap -> Exp {} -> (Heap -> Exp {} -> Prop) -> Prop where
+inductive Eval : Heap -> Exp {} -> Hpost -> Prop where
 | eval_val :
   (hv : Exp.IsVal v) ->
-  (hQ : Q h v) ->
+  (hQ : Q v h) ->
   Eval h v Q
 | eval_var :
-  (hQ : Q h (.var x)) ->
+  (hQ : Q (.var x) h) ->
   Eval h (.var x) Q
 | eval_apply {h : Heap} {x : Nat} :
   h x = some ⟨.abs T e, hv⟩ ->
@@ -26,30 +20,30 @@ inductive Eval : Heap -> Exp {} -> (Heap -> Exp {} -> Prop) -> Prop where
   h x = some ⟨.tabs T0 e, hv⟩ ->
   Eval h (e.subst (Subst.openTVar .top)) Q ->
   Eval h (.tapp (.free x) S) Q
-| eval_letin {h : Heap} {Q1 : Heap -> Exp {} -> Prop} :
-  (hpred : pred_is_monotonic Q1) ->  -- this local Q1 must be monotonic
+| eval_letin {h : Heap} {Q1 : Hpost} :
+  (hpred : Q1.is_monotonic) ->  -- this local Q1 must be monotonic
   Eval h e1 Q1 ->
   (h_val : ∀ {h1} {v : Exp {}},
     (hv : Exp.IsVal v) ->
-    Q1 h1 v ->
+    Q1 v h1 ->
     ∀ l', h1 l' = none ->
       Eval
         (h1.extend l' ⟨v, hv⟩)
         (e2.subst (Subst.openVar (.free l')))
         Q) ->
   (h_var : ∀ {h1} {x : Var {}},
-    Q1 h1 (.var x) ->
+    Q1 (.var x) h1 ->
     Eval h1 (e2.subst (Subst.openVar x)) Q) ->
   Eval h (.letin e1 e2) Q
 
 theorem eval_monotonic {h1 h2 : Heap}
-  (hpred : pred_is_monotonic Q)
+  (hpred : Q.is_monotonic)
   (hsub : h2.subsumes h1)
   (heval : Eval h1 e Q) :
   Eval h2 e Q := by
   induction heval generalizing h2
-  case eval_val => grind [Eval, pred_is_monotonic]
-  case eval_var => grind [Eval, pred_is_monotonic]
+  case eval_val => grind [Eval, Hpost.is_monotonic]
+  case eval_var => grind [Eval, Hpost.is_monotonic]
   case eval_apply hx _ ih =>
     specialize ih hpred hsub
     apply Eval.eval_apply
